hl|tc| 1. Mean and Variance
The Mean \(E[X]\) and Variance \(V[X]\) are numbers that measure the central value and spread of the distribution of a given random variable \(X\).
tc| \(E[X]=\sum_x xP(X=x)\)
tc| \(V[X] = \sum_x (x - E[X])^2 P(X=x) = E[(X-E[X])^2] = E[X^2] - E[X]^2 \)
Given two numbers \((a, b),\) we can compute (mean, variance) of the scaled and translated random variable \(aX+b\) as follows,
tc| \(E[aX+b] = aE[X]+b\)
tc| \(V[aX+b] = E[(aX+b-E[aX+b])^2] = E[a^2(X-E[X])^2] = a^2V[x]\)
Given two random variables \(X\) and \(Y\), the expectation and variance of \(X+Y\) can be computed with the same basic definitions as well,
tc| \( E[X+Y] = \sum_x \sum_y P(X=x) P(Y=y) (x+y)\)
tc| \( = \sum_x P(X=x) \sum_y P(Y=y) (x+y) \)
tc| \( = \sum_x P(X=x) \{x + E[Y]\} = E[X] + E[Y] \)
tc| \( V[X+Y] = E[(X+Y - E[X+Y])^2] = E[((X-E[X])+(Y-E[Y]))^2] \)
tc| \(= (V[X] + V[Y]) + 2E[(X-E[X])(Y-E[Y])] \)
If the random variables are independent, the covariance term in the variance of summation is zero, and the variance of the sum is the sum of varaince values. Note that variance scales quadratically when a random variable is scaled, but scales linearly when independent copies of the random variable are added to each other. The intuition behind this distinction is that when adding independent identical copies of a random variable, we allow destructive interference in the result which reduces the overall spread. The same does not happen with simple scaling.
We can also simplify these properties for the product of the given random variables assuming independence as follows,
tc| \( E[XY] = \sum_x \sum_y P(X=x)P(Y=y) xy = \sum_x P(X=x)x \sum_y P(Y=y)y = E[X]E[Y] \)
tc| \( V[XY] = E\left[ (XY-E[XY])^2 \right] = E\left[X^2Y^2 + E[X]^2 E[Y]^2 - 2XYE[X]E[Y] \right] = E[X^2]E[Y^2] - E[X]^2E[Y]^2 \)
tc| \( V[X]V[Y] = E\left[(X-E[X])^2(Y-E[Y])^2 \right] = E[X^2]E[Y^2] - E[X]^2E[Y^2] - E[X^2]E[Y]^2 + E[X]^2E[Y]^2 \)
Using the expansions of \(V[XY]\) and \(V[X]V[Y]\) above, we can observe the following,
tc| \( V[XY] = V[X]V[Y] + E[X^2]E[Y]^2 + E[X]^2E[Y^2] - 2E[X]^2E[Y]^2 \)
tc| \( V[XY] = V[X]V[Y] + V[X]E[Y]^2 + V[Y]E[X]^2 \)